\documentclass[a4paper, 10pt]{article}

% Encoding
\usepackage[T1]{fontenc}
\usepackage[utf8]{inputenc}
\usepackage[english]{babel}

% Margins
\usepackage[left=2.5cm, right=2.5cm]{geometry}

% Mathematics
\usepackage{amsmath, amssymb, mathtools, amsthm}

% Bibliography (uncomment if needed)
\usepackage{csquotes}
\usepackage[backend=biber, sorting=none, style=nature]{biblatex}
\addbibresource{biblio.bib}

% Personal taste
\usepackage[font=footnotesize]{caption}
\usepackage[parfill]{parskip}


\title{Some derivation of the axon problem}
\author{}

\begin{document}

  \maketitle

  This is about Nestor's diffusion advection problem. We have a finite axon of
  length $L$, with some influx $j_0$ at the soma ($x=0$). We also know that the
  dendrite is closed, so no net flux will be possible at $x=L$.\\
  Our chemical species $u : (x,t) \mapsto u(x,t)$ undergoes diffusion,
  advection, and decay. If I am not mistaken, the problem can be formulated as
  the initial boundary problem:

  \begin{equation}\label{eq:problem}
    \left\{ \begin{aligned}
      &u_t = D \, u_{xx} - v \, u_x - k \, u\\
      &\left[D \, u_x - v \, u\right]_{(0,t)} = j_0\\
      &\left[D \, u_x - v \, u\right]_{(L,t)} = 0\\
      &u(x,0) = \varphi(x)
    \end{aligned}\right.
  \end{equation}
  
  on the domain $x \in D = [0, L]$ and $t \in [0, +\infty]$.
  This is very classic stuff and I sure hope there exists a solution of
  some sort. Let us start first with the steady-state solution

  \paragraph{Steady-state} In order to find the steady-state solution
  $s(x) = u(x, t\to \infty)$, we impose $u_t = 0$. That leaves us with the
  Sturm-Liouville problem

  \begin{equation}
    \left\{\begin{aligned}
      &D s'' - v s' - k s = 0\\
      & D s'(0) - v s(0) = j0 \\
      & D s'(L) - v s(L) = 0 \\
    \end{aligned}\right.
  \end{equation}

  which admits the general solution
  
  \begin{equation}
    s(x) = a \, e^{\lambda_1 x} + b \, e^{\lambda_2 x}, \quad a, b \in \mathbb{R}
  \end{equation}

  Since $D, v, k > 0$ (things diffuse, move rightwards and degrade in time),
  also the eigenvalues $\lambda_1$ and $\lambda_2$ will be real.
  We can now proceed and find the exact values of $a$ and $b$ by direct
  substitution in the boundary conditions. Before going ahead, we rewrite the
  expressions for $s(x)$ and $s'(x)$ in the more convenient form

  \begin{align}
    &s(x) = e^{\frac{v}{2D}x}\left[a \, e^{\frac{\Delta}{2D}x} + b \,
      e^{-\frac{\Delta}{2D}x}\right]\\[6pt]
    &s'(x) = \frac{v}{2D}s(x) + \frac{\Delta}{2D} e^{\frac{v}{2D}x}\left[a \,
      e^{\frac{\Delta}{2D}x} - b \, e^{-\frac{\Delta}{2D}x}\right]
  \end{align}

  where $\Delta = \sqrt{v^2 + 4 D k}$. By inserting these expressions in the
  boundary conditions, we obtain

  \begin{equation*}
    \left\{\begin{aligned}
    &b = \frac{\Delta - v}{\Delta + v} \, a - \frac{2j_0}{\Delta - v}\\[6pt]
    &b = \exp\left\{\frac{\Delta}{D}L\right\} \, \frac{\Delta - v}{\Delta + v}
    \,a
    \end{aligned}\right.
  \end{equation*}

  This yields the constant values

  \begin{equation}
    a = \frac{2j_0}{(\Delta - v)(1-e^{\frac{\Delta}{D}L})},
    \qquad
    b = \frac{2j_0 \, e^{\frac{\Delta}{D}L}}
    {(\Delta + v)(1-e^{\frac{\Delta}{D}L})}
  \end{equation}
  
  and the final expression for $s(x)$ as
  \begin{equation}
    s(x) = \frac{2j_0}{1-e^{\frac{\Delta}{D}L}} \, e^{\frac{v}{2D}x}
    \left[\frac{e^{\frac{\Delta}{2D}x}}{\Delta - v} +
    \frac{e^{-\frac{\Delta}{2D}(x-2L)}}{\Delta + v}\right]
  \end{equation}

  Interestingly, the flux $j_0$ acts as a scaling parameter.

  \paragraph{Full solution} I don't really know how to do this for now but soon.
  Below are some failed attempts. We start with the substitution

  \begin{equation}\label{eq:change}
    u(x,t) = w(x,t) \, e^{\eta t - \mu x}  
  \end{equation}

  where

  \begin{equation}
    \eta = k + \frac{v^2}{4D}, \qquad \mu = \frac{v}{2D}
  \end{equation}
  
  by direct substitution we get 

  \begin{equation}\label{eq:diffusion:w}
    \left\{ \begin{aligned}
      &w_t = D \, w_{xx}\\
      &D \, w_x(0, t)  - (D \mu + v) w(0,t)  = j_0 \, e^{-\eta t}\\
      &D \, w_x(L, t)  - (D \mu + v) w(L,t)  = 0\\
      &w(x,0) = \varphi(x) \, e^{\mu x - \eta t} 
    \end{aligned}\right.
  \end{equation}
  
  We have, therefore, a initial boundary problem for the diffusion of $w(x,t)$,
  with Robin boundary conditions that depend on time. To try and tackle this
  problem, we will follow the recipe in \cite{Drbek2007ElementsOP} and
  integrating it with \cite{Salsa2022PartialDE}.\\ 
  We start by separating our solution $w(x,t)$ in two parts, one denominated
  $S(x,t)$, representing the steady-state of \eqref{eq:diffusion:w}, and the
  other $U(x,t)$ representing the transient perturbation of $w(x,t)$ from its
  asymptotic steady state

  \begin{equation}
    w(x,t) = S(x,t) + U(x,t)
  \end{equation}
  
  By construction, $S(x,t)$ has to respect the boundary value problem
  \eqref{eq:diffusion:w} for $t \to \infty$. Following, without any pretentions
  of originality, the method illustrated in \cite{Drbek2007ElementsOP}, we posit
  for $S(x,t)$ the following ``quasi-steady-state'' form

  \begin{equation}
    S(x,t) = A(t) \left(1 - \frac{x}{l}\right) + B(t)\frac{x}{l}
  \end{equation}

  The two unknown functions can be promptly found by substituting $S(x,t)$ in
  the boundary conditions

  \begin{equation}
    \left\{\begin{aligned}
      &\frac{D}{l}\left(B-A\right) - \frac{3}{2}v A = j_0e^{-\eta t}\\
      &\frac{D}{l}\left(B-A\right) - \frac{3}{2}v B = 0
    \end{aligned}\right.
  \end{equation}

  obtaining
  
  \begin{equation}
    A(t) = \left[\frac{2D}{3lv}-1\right]\frac{2 j_0}{3 v} e^{-\eta t}, \quad
    B(t) = \frac{4D j_0}{9 l v^2} e^{-\eta t}
  \end{equation}

  and therefore 

  \begin{equation}
    S(x,t) = \left[\frac{x}{l} + \frac{2D}{3lv} - 1\right] \frac{2
    j_0}{3v}e^{-\eta t}
  \end{equation}

  After finding $S(x,t)$, we can correctly define the problem for the transient
  solution $U(x,t)$, subject to Dirichlet boundary conditions:

  \begin{equation}
    \left\{ \begin{aligned}
      &U_t = D U_{xx}\\
      &D \, U_x(0, t)  - \frac{3}{2} U(0,t)  = 0\\
      &D \, U_x(L, t)  - \frac{3}{2} U(L,t)  = 0\\
      &U(x,0) = \varphi(x)e^{\mu x - \eta t} - S(x,0) =:\tilde{\varphi}(x)
    \end{aligned}\right.
  \end{equation}

  We can proceed with separation of variables, and posit that $U(x,t) =
  X(x)T(t)$. We first solve the spatial boundary value problem

  \begin{equation}
    \left\{\begin{aligned}
      &X'' + \lambda X = 0\\
      &D \, X'(0)  - \frac{3}{2} X(0)  = 0\\
      &D \, X'(L)  - \frac{3}{2} X(L)  = 0\\
    \end{aligned}\right.
  \end{equation}

  The only non-trivial solution of this BVP can be written, assuming $\lambda >
  0$, as

  \begin{equation}
    X(x) = a \cos \sqrt{\lambda} x + b \sin \sqrt{\lambda} x 
  \end{equation}

  and obtain the values for $\lambda$ and the relationship between $a$ and
  $b$ by substituting in the boundary conditions

  \begin{align}
    &\left\{\begin{aligned}
      &D b \sqrt{\lambda} - \frac{3}{2}v a = 0\\
      &D\sqrt{\lambda} \left[b \cos \sqrt{\lambda} l - a \sin \sqrt{\lambda}
      l\right] - \frac{3}{2}v \left[a\cos \sqrt{\lambda} l + b \sin
      \sqrt{\lambda}l\right] = 0
    \end{aligned}\right.\\[6pt]
    %
    &\left\{\begin{aligned}
      &D b \sqrt{\lambda} - \frac{3}{2}v a = 0\\
      &\cos\sqrt{\lambda}l \left[Db\sqrt{\lambda} - \frac{3}{2}va\right] + \sin
      \sqrt{\lambda}l \left[Da\sqrt{\lambda} + \frac{3}{2}v b \right] = 0
    \end{aligned}\right.\\[10pt]
    %
    &\left\{\begin{aligned}
      & a = \frac{2 D b}{3v} \sqrt{\lambda}\\
      &\frac{b}{6v} \sin \sqrt{\lambda} l \left[4D^2 \lambda + 9 v^2\right] = 0
    \end{aligned}\right.
  \end{align}

  Since $\lambda > 0$, its only possible values are $\lambda = \frac{n^2
  \pi^2}{l}$, $n \in \mathbb{N}$, yielding the final form for $X(x)$ is

  \begin{equation}
    X(x) = C_n \left[\frac{2 D n \pi}{3vl} \cos \frac{n \pi}{l}x + \sin \frac{n
    \pi}{l}x\right]
  \end{equation}



  \printbibliography

\end{document}





